sketchScript.sml
@@ -1,6 +1,6 @@
 open HolKernel boolLib bossLib lcsymtacs
 open miscLib pairSyntax stringSyntax listSyntax holSyntaxSyntax
-open pred_setTheory setSpecTheory holSyntaxTheory holSemanticsTheory holSemanticsExtraTheory
+open reflectionTheory pred_setTheory setSpecTheory holSyntaxTheory holSemanticsTheory holSemanticsExtraTheory
 
 val _ = temp_tight_equality()
 val _ = new_theory"sketch"
@@ -44,121 +44,6 @@ fun term_to_deep tm =
         mk_Abs(fromMLstring x, type_to_deep ty, term_to_deep b)
       end
 
-val mem = ``mem:'U->'U->bool``
-
-val ext_def = Define`
-  ext0 ^mem s = { a | mem a s }`
-val _ = Parse.overload_on("ext",``ext0 ^mem``)
-
-val finv_def = Define`
-  finv f x = @y. f y = x`
-
-val range_def = Define`
-  range0 ^mem (f : α -> 'U) = @x. BIJ f UNIV {a | mem a x}`
-val _ = Parse.overload_on("range",``range0 ^mem``)
-
-val in_bool_def = Define`
-  in_bool0 ^mem = Boolean`
-val _ = Parse.overload_on("in_bool",``in_bool0 ^mem``)
-
-val is_in_def = Define`
-  is_in0 ^mem f = ∃x. BIJ f UNIV {a | mem a x}`
-val _ = Parse.overload_on("is_in",``is_in0 ^mem``)
-
-val is_in_in_bool = store_thm("is_in_in_bool",
-  ``is_set_theory ^mem ⇒
-    is_in in_bool``,
-  rw[is_in_def,BIJ_IFF_INV] >>
-  qexists_tac`boolset` >>
-  rw[in_bool_def,boolean_in_boolset] >>
-  qexists_tac`λx. x = True` >>
-  rw[in_bool_def,boolean_eq_true] >>
-  rfs[mem_boolset,boolean_eq_true,true_neq_false,boolean_def])
-
-val in_fun_def = Define`
-  in_fun0 ^mem ina inb f =
-    Abstract (range ina) (range inb) (λx. inb (f (finv ina x)))`
-val _ = Parse.overload_on("in_fun",``in_fun0 ^mem``)
-
-val out_fun_def = Define`
-  out_fun0 ^mem ina inb mf x = finv inb (mf ' (ina x))`
-val _ = Parse.overload_on("out_fun",``out_fun0 ^mem``)
-
-val is_in_range_thm = store_thm("is_in_range_thm",
-  ``∀f. is_in f ⇒ BIJ f UNIV (ext (range f))``,
-  rw[is_in_def,range_def] >>
-  SELECT_ELIM_TAC >> conj_tac >- metis_tac[] >>
-  rw[ext_def])
-
-val is_in_finv_left = store_thm("is_in_finv_left",
-  ``∀ina.
-    is_in ina ⇒ ∀x. finv ina (ina x) = x``,
-  rw[finv_def] >>
-  SELECT_ELIM_TAC >>
-  conj_tac >-metis_tac[] >>
-  fs[is_in_def,BIJ_DEF,INJ_DEF])
-
-val is_in_finv_right = store_thm("is_in_finv_right",
-  ``∀ina.
-    is_in ina ⇒ ∀x. x <: range ina ⇒
-      (ina (finv ina x)) = x``,
-  rw[finv_def] >>
-  SELECT_ELIM_TAC >>
-  conj_tac >-(
-    imp_res_tac is_in_range_thm >>
-    fs[ext_def,BIJ_DEF,SURJ_DEF] ) >>
-  rw[])
-
-val is_in_in_fun = store_thm("is_in_in_fun",
-  ``is_set_theory ^mem ⇒
-    ∀ina inb. is_in ina ∧ is_in inb ⇒ is_in (in_fun ina inb)``,
-  rw[] >>
-  rw[is_in_def,BIJ_IFF_INV] >>
-  qexists_tac`Funspace (range ina) (range inb)` >>
-  conj_tac >- (
-    rw[in_fun_def] >>
-    match_mp_tac (UNDISCH abstract_in_funspace) >>
-    simp[range_def] >>
-    SELECT_ELIM_TAC >>
-    conj_tac >- metis_tac[is_in_def] >>
-    rw[] >>
-    SELECT_ELIM_TAC >>
-    conj_tac >- metis_tac[is_in_def] >>
-    rw[] >>
-    fs[BIJ_IFF_INV] ) >>
-  qexists_tac`out_fun ina inb` >>
-  conj_tac >- (
-    rw[out_fun_def,in_fun_def,FUN_EQ_THM] >>
-    qmatch_abbrev_tac`finv invb (Abstract s t f ' a) = Z` >>
-    rfs[] >>
-    `Abstract s t f ' a = f a` by (
-      match_mp_tac (UNDISCH apply_abstract) >>
-      imp_res_tac is_in_range_thm >>
-      fs[ext_def,BIJ_IFF_INV] >>
-      unabbrev_all_tac >> fs[] ) >>
-    rw[Abbr`Z`,Abbr`f`,Abbr`a`,Abbr`invb`] >>
-    imp_res_tac is_in_finv_left >>
-    simp[] ) >>
-  rw[in_fun_def,out_fun_def] >>
-  first_x_assum(mp_tac o
-    MATCH_MP(REWRITE_RULE[GSYM AND_IMP_INTRO](UNDISCH in_funspace_abstract))) >>
-  simp[AND_IMP_INTRO] >>
-  discharge_hyps >- (
-    imp_res_tac is_in_range_thm >>
-    fs[ext_def,BIJ_IFF_INV] >>
-    metis_tac[] ) >>
-  rw[] >>
-  match_mp_tac (UNDISCH abstract_eq) >>
-  gen_tac >>
-  qspecl_then[`f`,`ina (finv ina x)`,`range ina`,`range inb`]mp_tac
-    (UNDISCH apply_abstract) >>
-  discharge_hyps >- (
-    imp_res_tac is_in_range_thm >>
-    fs[ext_def,BIJ_DEF,INJ_DEF] ) >>
-  rw[] >>
-  imp_res_tac is_in_finv_right >>
-  rw[])
-
 fun underscores [] = ""
   | underscores (x::xs) = "_" ^ x ^ underscores xs
 
@@ -193,6 +78,7 @@ fun genv x =
   *)
   variant [] x
 
+val mem = ``mem:'U->'U->bool``
 val tysig = genv ``tysig:tyenv``
 val tmsig = genv ``tmsig:tmenv``
 val tyass = genv ``tyass:'U tyass``
@@ -214,12 +100,12 @@ val good_context_def = Define`
     is_valuation ^tysig ^tyass ^valuation`
 val good_context = good_context_def |> concl |> strip_forall |> snd |> lhs
 
-val Var_thm = store_thm("Var_thm",
+val Var_thm = prove(
   ``^tmval (x,ty) = inty v ⇒
     ∀mem. inty v = termsem0 mem ^tmsig (^tyass,^tmass) (^tyval,^tmval) (Var x ty)``,
   rw[termsem_def])
 
-val Const_thm = store_thm("Const_thm",
+val Const_thm = prove(
   ``instance ^tmsig ^interpretation name ty ^tyval = inty c ⇒
     ∀mem. inty c = termsem0 mem ^tmsig ^interpretation ^valuation (Const name ty)``,
   rw[termsem_def])
@@ -228,7 +114,7 @@ val instance_tm = Term.inst[alpha|->``:'U``]``instance``
 fun mk_instance name ty =
   list_mk_comb(instance_tm,[tmsig,interpretation,name,ty,tyval])
 
-val Comb_thm = store_thm("Comb_thm",
+val Comb_thm = prove(
   ``^good_context ⇒
     in_fun ina inb f = termsem ^tmsig ^interpretation ^valuation ftm ∧
     ina x = termsem ^tmsig ^interpretation ^valuation xtm ⇒
@@ -249,7 +135,7 @@ val Comb_thm = store_thm("Comb_thm",
   match_mp_tac is_in_finv_left >>
   simp[]) |> UNDISCH
 
-val Abs_thm = store_thm("Abs_thm",
+val Abs_thm = prove(
   ``^good_context ⇒
     ∀ina inb f x ty b.
     range ina = typesem tyass tyval ty ⇒
