simpleReflectionScript.sml
@@ -1,0 +1,75 @@
+open HolKernel boolLib bossLib lcsymtacs listTheory finite_mapTheory alistTheory pred_setTheory pairTheory
+open miscLib miscTheory setSpecTheory setModelTheory holSyntaxLibTheory holSyntaxTheory holSyntaxExtraTheory holSemanticsTheory holSemanticsExtraTheory
+
+val _ = temp_tight_equality()
+val _ = new_theory"simpleReflection"
+
+val mem = ``mem:'U->'U-> bool``
+val indin = ``indin:ind->'U``
+
+datatype simple_type = Ind | Bool | Fun of simple_type * simple_type
+
+fun type_name Ind = "ind"
+  | type_name Bool = "bool"
+  | type_name (Fun (s,t)) = "fun_" ^ type_name s ^ "_" ^ type_name t
+
+fun type_type Ind = mk_type("ind",[])
+  | type_type Bool = mk_type("bool",[])
+  | type_type (Fun (s,t)) = (type_type s --> type_type t) : hol_type
+
+
+fun set_type t = let val u = mk_vartype("'U") in
+  (u --> u --> mk_type("bool",[])) --> (mk_type("ind",[]) --> u)
+                                   --> u
+end
+
+fun in_type t = let val u = mk_vartype("'U") in
+  (u --> u --> mk_type("bool",[])) --> (mk_type("ind",[]) --> u)
+                                   --> type_type t --> u
+end
+
+fun out_type t = let val u = mk_vartype("'U") in
+  (u --> u --> mk_type("bool",[])) --> (mk_type("ind",[]) --> u)
+                                   --> u --> type_type t
+end
+
+fun set_var t = mk_var ("set_" ^ type_name t, set_type t)
+fun in_var t = mk_var ("in_" ^ type_name t, in_type t)
+fun out_var t = mk_var ("out_" ^ type_name t, out_type t)
+
+fun set_const t = mk_const ("set_" ^ type_name t, set_type t)
+fun in_const t = mk_const ("in_" ^ type_name t, in_type t)
+fun out_const t = mk_const ("out_" ^ type_name t, out_type t)
+
+fun set_expr Bool = `set_bool ^mem ^indin = boolset`
+  | set_expr Ind = `
+      set_ind ^mem ^indin = @indset. (!i. mem (indin i) indset)
+                                  /\ (!x. mem x indset ==> ?i. x = indin i)`
+  | set_expr (Fun (s,t)) = `
+      ^(set_var (Fun (s,t))) ^mem ^indin =
+        Funspace (^(set_const s) mem indin) (^(set_const t) mem indin)`
+
+fun in_expr Bool =
+      `(in_bool ^mem ^indin T = True) /\ (in_bool ^mem ^indin F = False)`
+  | in_expr Ind =
+      `in_ind ^mem ^indin i = indin i`
+  | in_expr (Fun (s,t)) =
+      `^(in_var (Fun (s,t))) ^mem ^indin f =
+           Abstract (^(set_const s) mem indin) (^(set_const t) mem indin) \x.
+             ^(in_const t) mem indin (f (^(out_const s) mem indin x))`
+
+fun out_expr t =
+  `^(out_var t) ^mem ^indin x = @y. ^(in_const t) mem indin y = x`
+
+fun mk t = ( xDefine ("set_" ^ type_name t) (set_expr t)
+           , xDefine ("in_" ^ type_name t) (in_expr t)
+           , xDefine ("out_" ^ type_name t) (out_expr t) )
+
+val res1 = mk Bool;
+val res2 = mk Ind;
+val res3 = mk (Fun (Bool,Bool));
+val res4 = mk (Fun (Ind,Ind));
+val res5 = mk (Fun (Ind,Bool));
+val res6 = mk (Fun (Fun (Ind,Ind), Fun (Ind,Bool)));
+
+val _ = export_theory()
